REPORT.md
@@ -2,9 +2,18 @@
 % Liewe Thomas van Binsbergen; João Paulo Pizani Flor;
 % July 5th, 2013
 
+# Accompanied files:
+* Main.v (containing the main function and proof)
+* SInc.v (containing the proves needed for 'fold_right step []')
+* Minimum.v (containing the proves about 'foldl1 join')
+* Tree.v (defining (functions on) trees)
+* Helpers.v (defining some helper lemmas that come in handy in the other files)
+* FoldStep.v (trying to define 'fold_right step []' as a single function)
+* Function.v (trying to define 'step' using the 'Function' keyword)
+
 # Introduction
 The functional Pearl "On Building Trees of Minimum Height" by Richard S. Bird
-solves the problem of building a tree out of a list of subtrees, in such a 
+solves the problem of building a tree out of a list of sub-trees, in such a 
 way that the resulting tree has the input list as its frontier while being
 minimum in the sense that any tree that we can build with this property has at
 least the same height. Where the height of a tree is defined as the maximum
@@ -35,11 +44,11 @@ single element) into a single tree. Since we show that for any strictly
 increasing list, the left-most pair is always an lmp, using 'foldl join' on
 this list will create a tree of minimal height.
 
-> build = foldl1 join . foldr step []
+> build = foldl1 join . fold_right step []
 
 In order to prove the correctness of this algorithm we will split up the work
 in two phases (each on one end of the function composition operator): 
-* First that 'foldr step []' produces a strictly increasing list
+* First that 'fold_right step []' produces a strictly increasing list
 * Second that 'foldl1 join', given a strictly increasing list, produces a 
 tree of minimum height.
 
@@ -51,22 +60,44 @@ an lmp, when given a strictly increasing list
 * Proving that 'foldl1 join' produces a tree of minimal height, when given
 a strictly increasing list 
 
-Both approaces will be equally correct, however in the first approach the
+Both approaches will be equally correct, however in the first approach the
 link between 'Lemma 1' and 'foldl1 join' is not explicit (only implied).
 This, however, makes it easier to prove, due to separation of concerns.
+
+We assume that the definition of fold_left that we have imported is indeed 
+correct.
+The loop 'foldl1 join' will always use join, unless the input list contains
+but a single element. From the definition of fold_left we know that 'fold join'
+will always join the first pair of a list. All we have to show is that
+every join operation performed by fold_left is 'safe' (invariant). 
+Where a safe join means that the joined pair is a local minimum pair in the
+given input list. Which comes down to showing that the left-most pair
+in a strictly increasing list is always an lmp and that appending
+the join of the left-most pair of a strictly increasing list preserves the
+fact that the left-most pair of this list is an lmp even though a list
+produced this way does not necessarily have to be strictly increasing anymore.
+
+The proofs can be found in the file Minimum.v.v and are named s_inc_leftmost_lmp 
+and join_preserves_leftmost_lmp.
+'Lemma 1' can also be found at this location(TODO).
 
 ## Definitions
 We have defined foldl1 (which is usually not total) using a predicate that
 the input list is not empty, which allows us to ignore the usual base case
 of foldl.
 
+TODO:
+* Prove 'foldl1 join => minimum' using 'Lemma 1' and a definition of 'minimum'
+explicitly, in such a way that it can be used in the proof for function
+'build'.
+
 # Proving strictly increasingness
-In order to prove that 'foldr step []' produces strictly increasing list we
+In order to prove that 'fold_right step []' produces strictly increasing list we
 will have to do case analysis on the function step.
 
 Function step acts very much like the list constructor 'cons', accept that
-it analyses the first elements of the list that it will add to.
-In order to do this the function must pattern match on the list.
+it analyzes the first elements of the list that it will add to by pattern 
+matching.
 When the newly element is smaller then the element currently on top of the list
 we can just add it, otherwise we will join the new element and the head of the
 list together and add this joined tree to the list instead (again using step).
@@ -77,6 +108,79 @@ single tree since join will be applied to all elements.
 Using 'join' is only safe (looking at the properties that the entire
 algorithm should have) when the joined pair is an lmp. And we can not 
 guarantee this when only looking at the first element of the list.
-We can, however, ensure this when we analyse the first two elements of the 
+We can, however, ensure this when we analyze the first two elements of the 
 list.
+ 
+In order to define the function step, which uses nested recursion and is 
+therefor not clearly structural decreasing, we have tried several methods for
+defining 'general recursion'. Including
+* Using the keyword 'Function'
+* Define 'fold_right step []' as a single function, since fold_right has a an
+obvious decreasing argument.
+* Using the Bove-Capretta method.
+* Using Well-foundedness (TODO)
+* Using a decreasing natural number and ensuring that it is always at least
+as big as the length of the input list of which we know that is decreases.
+We pattern match on this natural number and give a bogus result when it is 
+zero. Meaning that if we want to prove that the function step as certain 
+properties it can not return this bogus result.
+This corresponds very much to an amortizing argument, giving the function
+step a limit on the number of recursive calls it can use.
 
+Using the keyword 'Function' seemed like a very good approach since we 
+expected to be able to 'measure length input', where 'input' is the input list.
+However, 'Function' can not be used to define functions with nested recursion
+(a recursive call of which the result is an argument to a recursive call).
+(The attempt can be found in Function.v)
+
+The same problem we encountered when using the Bove-Capretta method. 
+Similar to their example about QuickSort in their paper on 'General Recursion',
+they provided an example of a function that has a nested recursive call.
+Bove and Capretta described in their paper a problem about nested recursive
+calls, namely that the predicate and function we want to define depend on each 
+other mutually. This is exactly the problem we encountered while defining the 
+function 'step'. The provided solution in the paper is based on work of 
+Dybjer (2000), who introduced a method of defining a predicate and the 
+definition it supports at the same time, even though they depend on each other.
+This method does, however, not help us to define the function / predicate pair
+in Coq.
+
+Another unsuccessful approach was trying to define 'fold_right step []'  as a
+single function (see FoldStep.v). The function is defined as to have two
+list of trees as arguments. One being the 'worklist', while the other is the
+'accumulated result'. When the worklist is empty we simply return the 
+accumulated result, otherwise we add the first element to the worklist
+to the accumulated result in such a way that it should match to definition of
+step in the paper by Bird. This new accumulated result is then given as an 
+argument to a recursive call of the function 'fold_step' together with the
+decreased worklist.
+When we reach the cases of the function step where we need a nested recursive
+call, due to the nature of the definition of 'fold_step', we have to invent
+a new worklist which contains only a single element.
+This seems to be the problem of this definition, since we have no assurance
+that the worklist of the current function call is actually larger then a 
+single element. Which means that we can not be sure that the input list
+is always structurally decreasing, since the old and the new worklist
+can both be of length one.
+
+A method that we did use successfully, was to use something very similar to an
+amortizing argument. Namely we give the function step a natural number as
+additional argument and make sure that this number is always decreased when
+being passed on with every recursive call. In order to assure that this can
+happen we need to pattern match on it and provide a function result when
+the natural number reaches zero. The result we give in this case is arbitrary
+and to prevent this result from ever being returned we must give the initial
+call a value high enough natural number to begin with.
+This number has to be related to the length of the input list and can not be
+arbitrary since we always increase the size of the input list to such an 
+extent that any arbitrary number is not enough. However, we can see, by 
+analyzing the algorithm (the paper suggests an amortizing approach), that the
+input list decreases at least by one in every recursive call. And since our
+natural number will exactly decrease by one every recursive call, we can 
+use the length of the input list as the initial value of this extra argument.
+
+Well-founded recursion (TODO)
+
+TODO: 
+* Prove the fact that 'fold step []' produces (anything non-empty)
+* Prove the fact that 'fold step []' produces a strictly increasing list
